messageInvariantPrototypes/shardedKv/distributedMonotonic/messageInvariants.dfy
@@ -1,0 +1,72 @@
+include "spec.dfy"
+
+module MessageInvariants {
+import opened Types
+import opened UtilitiesLibrary
+import opened MonotonicityLibrary
+import opened DistributedSystem
+
+ghost predicate SendReconfValidity(c: Constants, v: Variables)
+  requires v.WF(c)
+  requires ValidMessages(c, v)
+{
+  forall msg | msg in v.network.sentMsgs && msg.Reconf?
+  ::
+  (exists i ::
+    && v.ValidHistoryIdxStrict(i)
+    && Host.SendReconf(c.hosts[msg.Src()], v.History(i).hosts[msg.Src()], v.History(i+1).hosts[msg.Src()], msg)
+  )
+}
+
+ghost predicate MessageInv(c: Constants, v: Variables)
+{
+  && v.WF(c)
+  && ValidVariables(c, v)
+  && SendReconfValidity(c, v)
+}
+
+// Base obligation
+lemma InitImpliesMessageInv(c: Constants, v: Variables)
+  requires Init(c, v)
+  ensures MessageInv(c, v)
+{
+  InitImpliesValidVariables(c, v);
+}
+
+// Inductive obligation
+lemma MessageInvInductive(c: Constants, v: Variables, v': Variables)
+  requires MessageInv(c, v)
+  requires Next(c, v, v')
+  ensures MessageInv(c, v')
+{
+  InvNextValidVariables(c, v, v');
+  InvNextSendReconfValidity(c, v, v');
+}
+
+/***************************************************************************************
+*                                     Aux Proofs                                       *
+***************************************************************************************/
+
+
+lemma InvNextSendReconfValidity(c: Constants, v: Variables, v': Variables)
+  requires v.WF(c)
+  requires ValidMessages(c, v)
+  requires SendReconfValidity(c, v)
+  requires Next(c, v, v')
+  ensures SendReconfValidity(c, v')
+{
+  forall msg | msg in v'.network.sentMsgs && msg.Reconf?
+  ensures
+  (exists i ::
+    && v'.ValidHistoryIdxStrict(i)
+    && Host.SendReconf(c.hosts[msg.Src()], v'.History(i).hosts[msg.Src()], v'.History(i+1).hosts[msg.Src()], msg)
+  ) {
+    if msg !in v.network.sentMsgs {
+      // witness and trigger
+      var i := |v.history|-1;
+      assert Host.SendReconf(c.hosts[msg.Src()], v'.History(i).hosts[msg.Src()], v'.History(i+1).hosts[msg.Src()], msg);
+    }
+  }
+}
+
+} // end module MessageInvariants
