messageInvariantPrototypes/shardedKv/distributedMonotonic/ownershipInvariants.dfy
@@ -1,0 +1,198 @@
+include "spec.dfy"
+
+module OwnershipInvariants {
+  import opened Types
+  import opened UtilitiesLibrary
+  import opened DistributedSystem
+
+  ghost predicate KeyInFlight(c: Constants, v: Variables, k: OwnedKey) 
+    requires v.WF(c)
+  {
+    exists msg :: KeyInFlightByMessage(c, v, msg, k)
+  }
+
+  ghost predicate KeyInFlightByMessage(c: Constants, v: Variables, msg: Message, k: OwnedKey) 
+    requires v.WF(c)
+  {
+    && msg in v.network.sentMsgs
+    && (0 <= msg.Dst() < |c.hosts| ==>
+      Host.OwnedKeyInFlight(c.hosts[msg.Dst()], v.Last().hosts[msg.Dst()], k, msg)
+    )
+  }
+
+  ghost predicate AtMostOneInFlight(c: Constants, v: Variables)
+    requires v.WF(c)
+  {
+    forall k, m1, m2 | KeyInFlightByMessage(c, v, m1, k) && KeyInFlightByMessage(c, v, m2, k) 
+    :: m1 == m2
+  }
+
+  ghost predicate NoHostOwnsKey(c: Constants, v: Variables, k: OwnedKey) 
+    requires v.WF(c)
+  {
+    forall idx | c.ValidIdx(idx) :: !Host.HostOwnsKey(c.hosts[idx], v.Last().hosts[idx], k)
+  }
+
+  ghost predicate HostOwnsKeyImpliesNoneInFlight(c: Constants, v: Variables)
+    requires v.WF(c)
+  {
+    forall k | !NoHostOwnsKey(c, v, k)
+    ::
+    !KeyInFlight(c, v, k)
+  }
+
+  ghost predicate AtMostOwnedByOneHost(c: Constants, v: Variables)
+    requires v.WF(c)
+  {
+    forall h1, h2, k | 
+      && c.ValidIdx(h1) 
+      && c.ValidIdx(h2)
+      && Host.HostOwnsKey(c.hosts[h1], v.Last().hosts[h1], k) 
+      && Host.HostOwnsKey(c.hosts[h2], v.Last().hosts[h2], k) 
+    ::
+     h1 == h2
+  }
+
+  
+  ghost predicate OwnershipInv(c: Constants, v: Variables)
+  {
+    && v.WF(c)
+    && AtMostOneInFlight(c, v)
+    && AtMostOwnedByOneHost(c, v)
+    && HostOwnsKeyImpliesNoneInFlight(c, v)
+  }
+
+  lemma InitImpliesOwnershipInv(c: Constants, v: Variables)
+    requires Init(c, v)
+    ensures OwnershipInv(c, v)
+  {}
+
+  lemma OwnershipInvInductive(c: Constants, v: Variables, v': Variables)
+    requires OwnershipInv(c, v)
+    requires Next(c, v, v')
+    ensures OwnershipInv(c, v')
+  {
+    InvNextAtMostOneInFlight(c, v, v');
+    InvNextLiveKeyImpliesNoneInFlight(c, v, v');
+    InvNextAtMostOwnedByOneHost(c, v, v');
+  }
+
+
+/***************************************************************************************
+*                                 InvNext Proofs                                       *
+***************************************************************************************/
+
+
+lemma InvNextAtMostOneInFlight(c: Constants, v: Variables, v': Variables)
+  requires v'.WF(c)
+  requires OwnershipInv(c, v)
+  requires Next(c, v, v')
+  ensures AtMostOneInFlight(c, v')
+{
+  forall k, m1, m2 | KeyInFlightByMessage(c, v', m1, k) && KeyInFlightByMessage(c, v', m2, k) 
+  ensures m1 == m2
+  {
+    if m1 != m2 {
+      if KeyInFlightByMessage(c, v, m1, k) {
+        InvNextAtMostOneInFlightHelper(c, v, v', m1, m2, k);
+      } else {
+        InvNextAtMostOneInFlightHelper(c, v, v', m2, m1, k);
+      }
+    }
+  }
+}
+
+lemma InvNextAtMostOneInFlightHelper(c: Constants, v: Variables, v': Variables, m1: Message, m2: Message, k: OwnedKey)
+  requires v'.WF(c)
+  requires OwnershipInv(c, v)
+  requires Next(c, v, v')
+  // input constraints
+  requires m1 != m2
+  requires KeyInFlightByMessage(c, v, m1, k)
+  requires !KeyInFlightByMessage(c, v, m2, k)
+  // postcondition
+  ensures !KeyInFlightByMessage(c, v', m2, k)
+{
+  assert KeyInFlight(c, v, k);
+}
+
+lemma InvNextLiveKeyImpliesNoneInFlight(c: Constants, v: Variables, v': Variables)
+  requires v'.WF(c)
+  requires OwnershipInv(c, v)
+  requires Next(c, v, v')
+  ensures HostOwnsKeyImpliesNoneInFlight(c, v')
+{
+  forall k | !NoHostOwnsKey(c, v', k)
+  ensures !KeyInFlight(c, v', k)
+  {
+    forall msg | msg in v'.network.sentMsgs
+    ensures !KeyInFlightByMessage(c, v', msg, k) {
+      var idx :| c.ValidIdx(idx) && Host.HostOwnsKey(c.hosts[idx], v'.Last().hosts[idx], k);
+      if Host.HostOwnsKey(c.hosts[idx], v.Last().hosts[idx], k){
+        // triggers
+        assert !KeyInFlight(c, v, k);
+        assert !KeyInFlightByMessage(c, v, msg, k);
+
+      } else {
+        if msg in v.network.sentMsgs && KeyInFlightByMessage(c, v, msg, k){
+          var dsStep :| NextStep(c, v.Last(), v'.Last(), v.network, v'.network, dsStep);
+          // triggers
+          assert KeyInFlightByMessage(c, v, dsStep.msgOps.recv.value, k);
+          assert KeyInFlight(c, v, k);
+        }
+        assert !KeyInFlightByMessage(c, v', msg, k);
+      }
+    }
+  }
+}
+
+lemma InvNextAtMostOwnedByOneHost(c: Constants, v: Variables, v': Variables) 
+  requires v'.WF(c)
+  requires OwnershipInv(c, v)
+  requires Next(c, v, v')
+  ensures AtMostOwnedByOneHost(c, v')
+{
+  forall h1, h2, k | 
+      && c.ValidIdx(h1) 
+      && c.ValidIdx(h2)
+      && Host.HostOwnsKey(c.hosts[h1], v'.Last().hosts[h1], k) 
+      && Host.HostOwnsKey(c.hosts[h2], v'.Last().hosts[h2], k) 
+  ensures
+     h1 == h2
+  {
+    if h1 != h2 {
+      if v.Last().hosts[h1].HasLiveKey(k) {
+        AtMostOneHostOwnsKey(c, v, v', k, h1, h2);
+      } else if v.Last().hosts[h2].HasLiveKey(k) {
+        AtMostOneHostOwnsKey(c, v, v', k, h2, h1);
+      }
+    }
+  }
+}
+
+
+lemma AtMostOneHostOwnsKey(c: Constants, v: Variables, v': Variables, k: OwnedKey, idx: HostId, other: HostId)
+  requires v.WF(c) && v'.WF(c)
+  requires OwnershipInv(c, v)
+  requires c.ValidIdx(idx)
+  requires c.ValidIdx(other)
+  requires idx != other
+  requires Host.HostOwnsKey(c.hosts[idx], v.Last().hosts[idx], k) 
+  requires !Host.HostOwnsKey(c.hosts[other], v.Last().hosts[other], k) 
+  requires Next(c, v, v')
+  ensures !Host.HostOwnsKey(c.hosts[other], v'.Last().hosts[other], k) 
+{
+  var dsStep :| NextStep(c, v.Last(), v'.Last(), v.network, v'.network, dsStep);
+  var actor, msgOps := dsStep.actor, dsStep.msgOps;
+  if actor == other {
+    var cs, s, s' := c.hosts[other], v.Last().hosts[other], v'.Last().hosts[other];
+    var step :| Host.NextStep(cs, s, s', step, msgOps);
+    if step.ReceiveStep? && Host.HostOwnsKey(c.hosts[other], v'.Last().hosts[other], k) {
+      // triggers
+      assert KeyInFlightByMessage(c, v, msgOps.recv.value, k);  
+      assert KeyInFlight(c, v, k);
+      assert false;
+    }    
+  }
+}
+} // end module ShardedKVProof
